coq/theories/demo/BootstrappingDemo.v
@@ -1,0 +1,58 @@
+From impboot Require Import functional.FunSyntax functional.FunValues.
+From impboot Require Import imperative.ImpSyntax.
+From Stdlib Require Import NArith.
+From Stdlib Require Import ZArith.
+From Stdlib Require Import Lists.List.
+From Stdlib Require Import Bool.
+From Stdlib Require Import String.
+Require Import coqutil.Word.Interface.
+Require Import coqutil.Word.Properties.
+Require Import coqutil.Datatypes.List.
+Import ListNotations.
+Require Import impboot.imp2asm.ImpToASMCodegen.
+Require Import Derive.
+Require Import Ltac2.Ltac2.
+Require Import impboot.automation.RelCompiler.
+Require Import impboot.automation.ltac2.UnfoldFix.
+Require Import impboot.automation.AutomationLemmas.
+From impboot Require Import automation.Ltac2Utils.
+From impboot Require Import functional.FunValues.
+From impboot Require Import functional.FunSemantics.
+From impboot Require Import fp2imp.FpToImpCodegen.
+From impboot Require Import assembly.ASMToString.
+From impboot Require Import imperative.Printing.
+From impboot Require Import parsing.Parser.
+
+Print c_add.
+
+Derive c_add_fp
+  in ltac2:(relcompile_tpe 'c_add_fp 'c_add []) 
+  as c_add_prog_proof.
+Proof.
+  time relcompile.
+Qed.
+Print c_add_fp.
+
+Example c_add_imp :=
+  (to_funs [c_add_fp]).
+
+Compute c_add_imp.
+
+Compute (
+  match c_add_imp with
+  | Some [p] => Some (
+    flatten (fst (c_fundef p 0 []))
+  )
+  | _ => None
+  end
+).
+
+Time Eval lazy in (
+  match c_add_imp with
+  | Some [p] => Some (
+    let asm := flatten (fst (c_fundef p 0 [])) in
+    instrs2str 0 asm
+  )
+  | _ => None
+  end
+).
