coq/theories/demo/FunBigStepDemo.v
@@ -1,0 +1,94 @@
+Require Import String Nat.
+
+Open Scope nat.
+
+Inductive natExpr: Type :=
+  | NEConst (n: nat)
+  | NEVar (x: string)
+  | NEAdd (e1 e2: natExpr)
+  | NESub (e1 e2: natExpr).
+
+Inductive cmd: Type :=
+  | WLSkip
+  | WLAssign (x: string) (e: natExpr)
+  | WLSeq (c1 c2: cmd)
+  | WLIf (e: natExpr) (c1 c2: cmd)
+  | WLWhile (e: natExpr) (body: cmd).
+
+Definition state := string -> nat.
+Inductive res: Type :=
+| State (s: state)
+| TimeOut.
+Definition empty_state: res := State (fun _ => 0).
+Definition state_add (s: res) (x: string) (v: nat): res :=
+  match s with
+  | TimeOut => TimeOut
+  | State s => State (
+    fun y => if String.eqb y x then v else s y
+  )
+  end.
+Definition bind (s: res) (f: state -> res): res :=
+  match s with
+  | TimeOut => TimeOut
+  | State st => f st
+  end.
+Notation "'let*' x := s1 'in' s2" :=
+  (bind s1 (fun x => s2))
+  (at level 60, right associativity).
+
+Fixpoint eval_natExpr (s: state) (e: natExpr): nat :=
+  match e with
+  | NEConst n => n
+  | NEVar x => s x
+  | NEAdd e1 e2 => eval_natExpr s e1 + eval_natExpr s e2
+  | NESub e1 e2 => eval_natExpr s e1 - eval_natExpr s e2
+  end.
+Definition eval_natExpr_res (r: res) (e: natExpr): nat :=
+  match r with
+  | TimeOut => 0
+  | State s => eval_natExpr s e
+  end.
+
+Fixpoint eval_cmd (EVAL_CMD: forall (r: res) (c: cmd), res) (r: res) (c: cmd): res :=
+  let eval_cmd := eval_cmd EVAL_CMD in
+  match c with
+  | WLSkip => r
+  | WLAssign x e =>
+    state_add r x (eval_natExpr_res r e)
+  | WLSeq c1 c2 =>
+    let* r1 := eval_cmd r c1 in
+    eval_cmd (State r1) c2
+  | WLIf e c1 c2 =>
+    if eval_natExpr_res r e =? 0 then
+      eval_cmd r c2
+    else
+      eval_cmd r c1
+  | WLWhile e body =>
+    if eval_natExpr_res r e =? 0 then
+      r
+    else
+      let* r1 := eval_cmd r body in
+      EVAL_CMD (State r1) (WLWhile e body)
+  end.
+
+Fixpoint EVAL_CMD (fuel: nat) (r: res) (c: cmd): res :=
+  match fuel with
+  | 0 => TimeOut
+  | S fuel' =>
+    eval_cmd (EVAL_CMD fuel') r c
+  end.
+
+Example test_cmd :=
+  WLSeq
+    (WLAssign "x" (NEConst 1))
+    (WLWhile (NEVar "x")
+      (WLSeq
+        (WLAssign "y" (NEVar "x"))
+        (WLAssign "x" (NESub (NEVar "x") (NEConst (1)))))).
+
+Eval lazy in (
+  match (eval_cmd (EVAL_CMD 10) empty_state test_cmd) with
+  | TimeOut => 0
+  | State s => s "y"%string
+  end
+).
