coq/theories/demo/RecursiveFunctionReificationDemo.v
@@ -1,0 +1,77 @@
+From impboot Require Import functional.FunSyntax functional.FunValues.
+From impboot Require Import imperative.ImpSyntax.
+From Stdlib Require Import NArith.
+From Stdlib Require Import ZArith.
+From Stdlib Require Import Lists.List.
+From Stdlib Require Import Bool.
+From Stdlib Require Import String.
+Require Import coqutil.Word.Interface.
+Require Import coqutil.Word.Properties.
+Require Import coqutil.Datatypes.List.
+Import ListNotations.
+Require Import impboot.imp2asm.ImpToASMCodegen.
+Require Import Derive.
+Require Import Ltac2.Ltac2.
+Require Import impboot.utils.Core.
+Require Import impboot.automation.RelCompiler.
+Require Import impboot.automation.ltac2.UnfoldFix.
+Require Import impboot.automation.AutomationLemmas.
+From impboot Require Import automation.Ltac2Utils.
+From impboot Require Import functional.FunValues.
+From impboot Require Import functional.FunSemantics.
+From impboot Require Import fp2imp.FpToImpCodegen.
+From impboot Require Import assembly.ASMToString.
+From impboot Require Import imperative.Printing.
+From impboot Require Import parsing.Parser.
+
+Fixpoint sum (n: nat): nat :=
+  match n with
+  | 0%nat => 0%nat
+  | S n' => n + sum n'
+  end.
+
+Theorem sum_equation: ltac2:(unfold_fix_type '@sum).
+Proof. unfold_fix_proof '@sum. Qed.
+
+Derive sum_prog
+  in ltac2:(relcompile_tpe 'sum_prog 'sum [])
+  as sum_prog_proof.
+Proof.
+  intros * prog_eq * Hlookup.
+  subst sum_prog.
+  ltac1:(match goal with
+  | H: ?g = FunSyntax.Defun ?nm ?args ?body |- _ =>
+    instantiate(1 := FunSyntax.Defun nm args _) in H; inversion H; clear H; subst body
+  end).
+  ltac1:(fix IH 1).
+  intros.
+  rewrite sum_equation.
+  eapply trans_app.
+  3: eauto.
+  2: reflexivity.
+  refine open_constr:(auto_nat_case
+  (* env *) ltac2:(eauto)
+  (* s *) s
+  (* x0 x1 x2 *) _ _ _
+  (* name *) "n1"
+  (* v0 *) n
+  (* v1 *) 0%nat
+  (* v2 *) (fun n => (S n + sum n)%nat)
+  (* eval v0 *) _
+  (* eval v1 *) _
+  ).
+  3,4,5: ltac1:(shelve).
+  1: eapply trans_Var.
+  1: unfold make_env; eauto with fenvDb.
+  destruct n.
+  1: eapply auto_nat_const.
+  eapply auto_nat_add.
+  1: eapply auto_nat_succ.
+  1: eapply trans_Var.
+  1: unfold make_env; eauto with fenvDb.
+  eapply trans_Call.
+  2: eauto.
+  eapply trans_Var.
+  1: unfold make_env; eauto with fenvDb.
+  (* time relcompile. *)
+Qed.
