coq/theories/demo/ReifyingNonStructuralRecursionDemo.v
@@ -1,0 +1,52 @@
+From impboot Require Import functional.FunSyntax functional.FunValues.
+From impboot Require Import imperative.ImpSyntax.
+From Stdlib Require Import NArith.
+From Stdlib Require Import ZArith.
+From Stdlib Require Import Lists.List.
+From Stdlib Require Import Bool.
+From Stdlib Require Import String.
+Require Import coqutil.Word.Interface.
+Require Import coqutil.Word.Properties.
+Require Import coqutil.Datatypes.List.
+Import ListNotations.
+Require Import impboot.imp2asm.ImpToASMCodegen.
+Require Import Derive.
+Require Import Ltac2.Ltac2.
+Require Import impboot.utils.Core.
+Require Import impboot.automation.RelCompiler.
+Require Import impboot.automation.ltac2.UnfoldFix.
+Require Import impboot.automation.AutomationLemmas.
+From impboot Require Import automation.Ltac2Utils.
+From impboot Require Import functional.FunValues.
+From impboot Require Import functional.FunSemantics.
+From impboot Require Import fp2imp.FpToImpCodegen.
+From impboot Require Import assembly.ASMToString.
+From impboot Require Import imperative.Printing.
+From impboot Require Import parsing.Parser.
+
+Open Scope nat.
+
+Definition nat_modulo1 (n1 n2: nat): nat :=
+  match n2 with
+  | 0%nat => 0
+  | S _ => n1 - n2 * (n1 / n2)
+  end.
+
+Remark gcd_oblig:
+  forall (a b: nat) (NE: b <> 0), nat_modulo1 a b < b.
+Proof.
+Admitted.
+
+Function gcd (a b: nat) (ACC: Acc lt b) {struct ACC}: nat :=
+  match Nat.eq_dec b 0 with
+  | left EQ => a
+  | right NE =>
+    gcd b (nat_modulo1 a b) (Acc_inv ACC (gcd_oblig a b NE))
+  end.
+
+Derive gcd_prog
+  in ltac2:(relcompile_tpe 'gcd_prog 'gcd ['nat_modulo1])
+  as gcd_prog_proof.
+Proof.
+  time relcompile.
+Qed.
