coq/theories/demo/SimpleReificationDemo.v
@@ -1,0 +1,65 @@
+From impboot Require Import functional.FunSyntax functional.FunValues.
+From impboot Require Import imperative.ImpSyntax.
+From Stdlib Require Import NArith.
+From Stdlib Require Import ZArith.
+From Stdlib Require Import Lists.List.
+From Stdlib Require Import Bool.
+From Stdlib Require Import String.
+Require Import coqutil.Word.Interface.
+Require Import coqutil.Word.Properties.
+Require Import coqutil.Datatypes.List.
+Import ListNotations.
+Require Import impboot.imp2asm.ImpToASMCodegen.
+Require Import Derive.
+Require Import Ltac2.Ltac2.
+Require Import impboot.utils.Core.
+Require Import impboot.automation.RelCompiler.
+Require Import impboot.automation.ltac2.UnfoldFix.
+Require Import impboot.automation.AutomationLemmas.
+From impboot Require Import automation.Ltac2Utils.
+From impboot Require Import functional.FunValues.
+From impboot Require Import functional.FunSemantics.
+From impboot Require Import fp2imp.FpToImpCodegen.
+From impboot Require Import assembly.ASMToString.
+From impboot Require Import imperative.Printing.
+From impboot Require Import parsing.Parser.
+
+Definition f1: nat :=
+  let/d n := 2%nat in
+  (n + 1)%nat.
+
+Derive f1_prog
+  in ltac2:(relcompile_tpe 'f1_prog 'f1 [])
+  as f1_prog_proof.
+Proof.
+  intros.
+  subst f1_prog.
+  ltac1:(match goal with
+  | H: ?g = FunSyntax.Defun ?nm ?args ?body |- _ =>
+    instantiate(1 := FunSyntax.Defun nm args _) in H; inversion H; clear H; subst body
+  end).
+  unfold f1.
+  eapply trans_app.
+  3: eauto.
+  2: reflexivity.
+  refine open_constr:(auto_let
+  (* env *) ltac2:(eauto)
+  (* x1 y1 *) _ _
+  (* s1 s2 s3 *) ltac2:(exact s) ltac2:(exact s) ltac2:(exact s)
+  (* v1 *) 2%nat
+  (* let_n *) "n"
+  (* f *) (fun n => n + 1)%nat
+  (* eval v1 *) _
+  (* eval f *) _
+  ).
+  1: typeclasses_eauto.
+  3,4: ltac1:(shelve).
+  (* eapply auto_let with (let_n := "n"). *)
+  1: eapply auto_nat_const.
+  intros; cbv beta.
+  eapply auto_nat_add.
+  1: eapply trans_Var; eauto with fenvDb.
+  eapply auto_nat_const.
+
+  (* time relcompile. *)
+Qed.
